src/tls/Crypto.AEAD.fsti
@@ -5,7 +5,6 @@ module Seq = FStar.Seq
 module EC = EverCrypt.AEAD
 module SC = Spec.AEAD
 module B = LowStar.Buffer
-module E = EverCrypt
 module U32 = FStar.UInt32
 module HS = FStar.HyperStack
 module HST = FStar.HyperStack.ST
@@ -47,6 +46,13 @@ let tag_len : (x: SC.alg) -> Tot (y: U32.t { U32.v y == SC.tag_length x }) =
   | AES128_CCM        -> 16ul
   | AES256_CCM        -> 16ul
 
+inline_for_extraction
+let iv_len = 12ul
+
+inline_for_extraction
+noextract
+let iv_length = 12
+
 val encrypt
   (#a: SC.supported_alg)
   (#phi: plain_pred)
@@ -54,6 +60,8 @@ val encrypt
   (plain: EC.plain_p a)
   (plain_len: U32.t {U32.v plain_len == B.length plain})
   (cipher: EC.cipher_p a) // cipher == iv ++ cipher ++ tag (see EverCrypt.AEAD.encrypt_st)
+  // FIXME: for now we assume that cipher already contains some iv, but at some point
+  // we should have `encrypt` randomly generate it and write it into cipher
 : HST.Stack EE.error_code
   (requires (fun h ->
     invariant h s /\
@@ -63,15 +71,20 @@ val encrypt
     B.loc_disjoint (footprint s) (B.loc_buffer plain) /\
     B.loc_disjoint (footprint s) (B.loc_buffer cipher) /\
     B.disjoint plain cipher /\
-    B.length cipher == B.length plain + 12 + SC.tag_length a
+    B.length cipher == B.length plain + iv_length + SC.tag_length a
   ))
   (ensures (fun h res h' -> 
     match res with
     | EE.InvalidKey ->
-      B.modifies B.loc_none h h'
+      B.modifies B.loc_none h h' // TODO: should be False, need to fix EverCrypt
     | EE.Success ->
-      B.modifies (B.loc_union (footprint s) (B.loc_buffer cipher)) h h' /\
-      invariant h' s
+      // FIXME: currently we assume iv already in cipher,
+      // at some point it should be randomly generated here
+      let iv = B.gsub cipher 0ul iv_len in
+      let cipher' = B.gsub cipher iv_len (B.len cipher `U32.sub` iv_len) in
+      B.modifies (B.loc_union (footprint s) (B.loc_buffer cipher')) h h' /\
+      invariant h' s /\
+      (F.ideal_AEAD == false ==> SC.encrypt (state_kv s) (B.as_seq h iv) Seq.empty (B.as_seq h plain) `Seq.equal` B.as_seq h' cipher')
     | _ -> False
   ))
 
@@ -79,7 +92,7 @@ val decrypt
   (#a: SC.supported_alg)
   (#phi: plain_pred)
   (s: state a phi) // key
-  (cipher: EC.cipher_p a) // cipher == iv ++ cipher ++ tag (see EverCrypt.AEAD.encrypt_st)
+  (cipher: EC.cipher_p a) // cipher == iv ++ cipher ++ tag (see EverCrypt.AEAD.decrypt_st)
   (cipher_len: U32.t { U32.v cipher_len == B.length cipher })
   (plain: EC.plain_p a)
 : HST.Stack EE.error_code
@@ -87,18 +100,27 @@ val decrypt
     invariant h s /\
     B.live h plain /\
     B.live h cipher /\
-    B.length cipher == B.length plain + 12 + SC.tag_length a /\
+    B.length cipher == B.length plain + iv_length + SC.tag_length a /\
     B.loc_disjoint (footprint s) (B.loc_buffer plain) /\
     B.loc_disjoint (footprint s) (B.loc_buffer cipher) /\
     B.disjoint plain cipher
   ))
   (ensures (fun h res h' ->
+    let iv' = B.gsub cipher 0ul iv_len in
+    let cipher' = B.gsub cipher iv_len (cipher_len `U32.sub` iv_len) in
     match res with
     | EE.InvalidKey ->
-      B.modifies B.loc_none h h'
-    | EE.Success
+      B.modifies B.loc_none h h' // TODO: should be False, need to fix EverCrypt
+    | EE.Success ->
+      B.modifies (B.loc_union (footprint s) (B.loc_buffer plain)) h h' /\
+      invariant h' s /\ (
+        if F.ideal_AEAD
+        then phi (B.as_seq h' plain)
+        else SC.decrypt (state_kv s) (B.as_seq h iv') Seq.empty (B.as_seq h cipher') == Some (B.as_seq h' plain)
+      )
     | EE.AuthenticationFailure ->
       B.modifies (B.loc_union (footprint s) (B.loc_buffer plain)) h h' /\
-      invariant h' s
+      invariant h' s /\
+      (F.ideal_AEAD == false ==> SC.decrypt (state_kv s) (B.as_seq h iv') Seq.empty (B.as_seq h cipher') == None)
     | _ -> False
   ))
